tla-tree/ImmutableDiskTreeRefinement.dfy
@@ -4,6 +4,7 @@ include "ImmutableDiskTreeInterpretation.dfy"
 module ImmutableDiskTreeRefinement {
 import opened KVTypes
 import opened TreeTypes
+import ImmutableDiskTreeImpl
 import opened ImmutableDiskTree
 import opened ImmutableDiskTreeInv
 import opened ImmutableDiskTreeHeight
@@ -11,17 +12,48 @@ import opened ImmutableDiskTreeInterpretation
 import opened MissingLibrary
 import CrashableMap
 
+type View = ImmutableDiskTreeImpl.View
+function DiskSize(k:Constants) : int { ImmutableDiskTreeImpl.DiskSize(k.impl) }
+function ROOT_ADDR() : TableAddress { ImmutableDiskTreeImpl.ROOT_ADDR() }
+
+predicate WFDiskState(k:Constants, s:Variables)
+{
+    && TreeDisk.WF(k.disk, s.disk)
+    && k.disk.size == DiskSize(k)
+}
+
+function {:opaque} DiskView(k:Constants, s:Variables) : (diskView:View)
+    requires WFDiskState(k, s)
+    ensures FullView(k.impl, diskView)
+    ensures forall lba :: 0 <= lba < DiskSize(k) ==> diskView[lba] == s.disk.sectors[lba]
+{
+    map lba | 0 <= lba < DiskSize(k) :: s.disk.sectors[lba]
+}
+
+// I rewritten from ImmutableDiskTree namespace.
+function Jk(k:Constants) : CrashableMap.Constants
+{
+    Ik(k.impl)
+}
+
+function J(k:Constants, s:Variables) : CrashableMap.Variables
+    requires WFDiskState(k, s)
+    requires TreeInv(k.impl, s.impl, DiskView(k, s))
+{
+    I(k.impl, s.impl, DiskView(k, s))
+}
+
 lemma InvImpliesRefinementInit(k:Constants, s:Variables)
     requires Init(k, s)
-    requires TreeInv(k, s)
-    ensures CrashableMap.Init(Ik(k), I(k, s))
+    requires TreeInv(k.impl, s.impl, DiskView(k, s))
+    ensures CrashableMap.Init(Jk(k), J(k, s))
 {
     reveal_ISubtreePrefixView();
     reveal_ISlotView();
-    var tv := PersistentTreeView(k, s);
+    var tv := PersistentTreeView(k.impl, DiskView(k, s));
     assert ISubtreeView(tv, ROOT_ADDR()) == ISubtreePrefixView(tv, ROOT_ADDR(), /*slotCount*/ 1); // OBSERVE
-    assert IPersistentView(k, s) == CrashableMap.EmptyMap(); // OBSERVE
-} 
+    assert IPersistentView(k.impl, DiskView(k, s)) == CrashableMap.EmptyMap(); // OBSERVE
+}
 
 function FetchStep(k:Constants, s:Variables, s':Variables) : (step:Step)
     requires Next(k, s, s')
@@ -34,18 +66,18 @@ function FetchStep(k:Constants, s:Variables, s':Variables) : (step:Step)
 
 lemma InvImpliesRefinementNext(k:Constants, s:Variables, s':Variables)
     requires Next(k, s, s')
-    requires TreeInv(k, s)
-    requires TreeInv(k, s')
-    ensures CrashableMap.WF(I(k, s))
-    ensures CrashableMap.WF(I(k, s'))
-    ensures CrashableMap.Next(Ik(k), I(k, s), I(k, s'))
+    requires TreeInv(k.impl, s.impl, DiskView(k, s))
+    requires TreeInv(k.impl, s'.impl, DiskView(k, s'))
+    ensures CrashableMap.WF(J(k, s))
+    ensures CrashableMap.WF(J(k, s))
+    ensures CrashableMap.Next(Jk(k), J(k, s), J(k, s'))
 {
-    var Ik := Ik(k);
-    var Is := I(k, s);
-    var Is' := I(k, s');
+    var Ik := Jk(k);
+    var Is := J(k, s);
+    var Is' := J(k, s');
     var step := FetchStep(k, s, s');
 
-    match step {
+    match step.impl {
         case QueryActionStep(lookup, datum) => {
             assert CrashableMap.Query(Ik, Is, Is', datum);
         }
